share/pulse/examples/NuPool.fsti
@@ -3,78 +3,88 @@ module NuPool
 open Pulse.Lib.Pervasives
 open Pulse.Lib.Par.Pledge
 module T = FStar.Tactics.V2
-
-noeq
-type vcode : Type u#3 = {
-    t : Type u#2;
-    up : t -> vprop;
-}
+open Codeable
 
 val handle : Type u#0
+val pool (code_t:Type u#2) : Type u#0
+val pool_alive (#[T.exact (`full_perm)] f : perm) (code:vcode) (p:pool code.t) : vprop
 
-
-val pool (code:vcode) : Type u#0
-val pool_alive (#[T.exact (`full_perm)] f : perm) (#code:vcode) (p:pool code) : vprop
-
-val joinable (#code:vcode) (p:pool code) (post:erased code.t) (h : handle) : vprop
+val joinable (#code_t:Type u#2) (p:pool code_t) (post:erased code_t) (h : handle) : vprop
 
 val spawn
   (#code:vcode)
-  (p : pool code)
+  (p : pool code.t)
   (#pf : perm)
   (#pre : erased code.t)
   (#post : erased code.t)
   (f : unit -> stt unit (code.up pre) (fun _ -> code.up post))
-  : stt handle (pool_alive #pf p ** code.up pre)
-               (fun h -> pool_alive #pf p ** joinable p post h)
+  : stt handle (pool_alive #pf code p ** code.up pre)
+               (fun h -> pool_alive #pf code p ** joinable p post h)
 
-val pool_done (#code:vcode) (p:pool code) : vprop
+val pool_done (code:vcode) (p:pool code.t) : vprop
 
 val disown
   (#code:vcode)
-  (#p : pool code)
+  (#p : pool code.t)
   (#post : erased code.t)
   (h : handle)
   : stt_ghost unit (joinable p post h)
-                   (fun _ -> pledge [] (pool_done p) (code.up post))
+                   (fun _ -> pledge [] (pool_done code p) (code.up post))
 
 (* spawn + disown *)
 val spawn_
   (#code:vcode)
-  (p : pool code)
+  (p : pool code.t)
   (#pf : perm)
   (#pre : erased code.t)
   (#post : erased code.t)
   (f : unit -> stt unit (code.up pre) (fun _ -> code.up post))
-  : stt unit (pool_alive #pf p ** code.up pre)
-             (fun _ -> pool_alive #pf p ** pledge [] (pool_done p) (code.up post))
+  : stt unit (pool_alive #pf code p ** code.up pre)
+             (fun _ -> pool_alive #pf code p ** pledge [] (pool_done code p) (code.up post))
 
 val await
   (#code:vcode)
-  (#p : pool code)
+  (#p : pool code.t)
   (#post : erased code.t)
   (h : handle)
   (#f : perm)
-  : stt unit (pool_alive #f p ** joinable p post h)
-             (fun _ -> pool_alive #f p ** code.up post)
+  : stt unit (pool_alive #f code p ** joinable p post h)
+             (fun _ -> pool_alive #f code p ** code.up post)
 
 val await_pool
   (#code:vcode)
-  (p:pool code)
+  (p:pool code.t)
+  (#is:Pulse.Lib.InvList.invlist)
   (#f:perm)
   (q : vprop)
-  : stt unit (pool_alive #f p ** pledge [] (pool_done p) q)
-             (fun _ -> pool_alive #f p ** q)
+  : stt unit (pool_alive #f code p ** pledge is (pool_done code p) q)
+             (fun _ -> pool_alive #f code p ** q)
 
 val teardown_pool
   (#code:vcode)
-  (p:pool code)
-  (#f:perm)
-  : stt unit (pool_alive #f p)
-             (fun _ -> pool_done p)
+  (p:pool code.t)
+  : stt unit (pool_alive code p)
+             (fun _ -> pool_done code p)
 
 val setup_pool
   (#code:vcode)
   (n : pos)
-  : stt (pool code) emp
-                    (fun p -> pool_alive p)
+  : stt (pool code.t)
+         emp
+         (fun p -> pool_alive code p)
+
+val share_alive
+  (#code:vcode)
+  (p:pool code.t)
+  (e:perm)
+  : stt_ghost unit
+              (pool_alive #e code p)
+              (fun () -> pool_alive #(half_perm e) code p ** pool_alive #(half_perm e) code p)
+
+val gather_alive
+  (#code:vcode)
+  (p:pool code.t)
+  (e:perm)
+  : stt_ghost unit
+              (pool_alive #(half_perm e) code p ** pool_alive #(half_perm e) code p)
+              (fun () -> pool_alive #e code p)
